Updated Smt-goal-generator.lisp with function expansion.

verified/SMT-goal-generator.lisp
@@ -9,55 +9,467 @@
 (include-book "std/util/bstar" :dir :system)
 (include-book "xdoc/top" :dir :system)
 (include-book "std/util/define" :dir :system)
+(include-book "ordinals/lexicographic-ordering" :dir :system)
+;; for lambda expression
+(include-book "kestrel/utilities/terms" :dir :system)
+;; for symbol-fix
+(include-book "centaur/fty/basetypes" :dir :system)
 
+;; Include SMT books
 (include-book "SMT-hint-interface")
+
 
 (defsection SMT-goal-generator
   :parents (Smtlink)
   :short "SMT-goal-generator generates the three type of goals for the verified
   clause processor"
 
-  (define expand (term hints)
-    :ignore-ok t
-    :irrelevant-formals-ok t
-    term)
+  (defalist sym-nat-alist
+    :key-type symbol
+    :val-type natp
+    :pred sym-nat-alistp
+    :true-listp t)
 
-  (define generate-fn-hint-lst (fn-lst)
-    :guard (func-listp fn-lst)
-    :returns (fn-hint-lst hint-pair-listp)
-    :ignore-ok t
-    :irrelevant-formals-ok t
+  (defthm consp-of-sym-nat-alist-fix
+    (implies (consp (sym-nat-alist-fix x)) (consp x))
+    :hints (("Goal" :in-theory (enable sym-nat-alist-fix))))
 
-    nil
+  (defthm len-of-sym-nat-alist-fix-<
+    (> (1+ (len x)) (len (sym-nat-alist-fix x)))
+    :hints (("Goal" :in-theory (enable sym-nat-alist-fix))))
+
+  (defthm natp-of-cdar-sym-nat-alist-fix
+    (implies (consp (sym-nat-alist-fix x))
+             (natp (cdar (sym-nat-alist-fix x))))
+    :hints (("Goal" :in-theory (enable sym-nat-alist-fix))))
+
+  (define update-fn-lvls ((fn symbolp) (fn-lvls sym-nat-alistp))
+    :returns (updated-fn-lvls sym-nat-alistp)
+    :measure (len fn-lvls)
+    :hints (("Goal" :in-theory (enable sym-nat-alist-fix)))
+    :enabled t
+    (b* ((fn (mbe :logic (symbol-fix fn) :exec fn))
+         (fn-lvls (mbe :logic (sym-nat-alist-fix fn-lvls) :exec fn-lvls))
+         ((unless (consp fn-lvls)) nil)
+         ((cons first rest) fn-lvls)
+         ((cons this-fn this-lvl) first)
+         ((unless (equal fn this-fn))
+          (cons (cons this-fn this-lvl)
+                (update-fn-lvls fn rest))))
+      (if (zp this-lvl)
+          (cons (cons this-fn 0) rest)
+        (cons (cons this-fn (1- this-lvl)) rest)))
+    ///
+    (more-returns
+     (updated-fn-lvls
+      (implies (and (symbolp fn)
+                    (sym-nat-alistp fn-lvls)
+                    (consp fn-lvls)
+                    (hons-get fn fn-lvls)
+                    (not (equal (cdr (hons-get fn fn-lvls)) 0)))
+               (< (cdr (assoc fn updated-fn-lvls))
+                  (cdr (assoc fn fn-lvls))))
+      :name updated-fn-lvls-decrease))
     )
 
-  (define generate-hyp-hint-lst (hyp-lst)
-    :guard (hint-pair-listp hyp-lst)
+  (define flatten-formals ((formal-lst decl-listp))
+    :returns (formals symbol-listp)
+    :measure (len formal-lst)
+    :hints (("Goal" :in-theory (enable decl-list-fix)))
+    :enabled t
+    (b* ((formal-lst (mbe :logic (decl-list-fix formal-lst) :exec formal-lst))
+         ((if (endp formal-lst)) nil)
+         ((cons first rest) formal-lst)
+         ((decl d) first))
+      (cons d.name (flatten-formals rest))))
+
+  (defprod ex-args
+    ((term-lst pseudo-term-listp :default nil)
+     (fn-lst func-alistp :default nil)
+     (fn-lvls sym-nat-alistp :default nil)))
+
+  (defthm natp-of-sum-lvls-lemma
+    (implies (and (consp (sym-nat-alist-fix fn-lvls)) (natp x))
+             (natp (+ (cdr (car (sym-nat-alist-fix fn-lvls))) x)))
+    :hints (("Goal"
+             :in-theory (enable sym-nat-alist-fix)
+             :use ((:instance natp-of-cdar-sym-nat-alist-fix)))))
+
+  (define sum-lvls ((fn-lvls sym-nat-alistp))
+    :returns (sum natp :hints (("Goal"
+                                :use ((:instance natp-of-sum-lvls-lemma
+                                                 (x (sum-lvls (cdr (sym-nat-alist-fix fn-lvls)))))))))
+    :measure (len fn-lvls)
+    :hints (("Goal" :in-theory (enable sym-nat-alist-fix)))
+    :enabled t
+    (b* ((fn-lvls (mbe :logic (sym-nat-alist-fix fn-lvls) :exec fn-lvls))
+         ((unless (consp fn-lvls)) 0)
+         ((cons first rest) fn-lvls)
+         ((cons & lvl) first))
+      (+ lvl (sum-lvls rest)))
+    ///
+    (defthm sum-lvls-decrease-after-update
+      (implies (and (symbolp fn)
+                    (sym-nat-alistp fn-lvls)
+                    (consp fn-lvls)
+                    (hons-get fn fn-lvls)
+                    (not (equal (cdr (hons-get fn fn-lvls)) 0)))
+               (< (sum-lvls (update-fn-lvls fn fn-lvls))
+                  (sum-lvls fn-lvls)))))
+
+  (define expand-measure ((expand-args ex-args-p))
+    :returns (m nat-listp)
+    :enabled t
+    (b* ((expand-args (mbe :logic (ex-args-fix expand-args) :exec expand-args))
+         ((ex-args a) expand-args)
+         (lvl-sum (sum-lvls a.fn-lvls)))
+      (list lvl-sum (acl2-count a.term-lst))))
+
+  (encapsulate ()
+    (local (defthm lemma-1
+             (implies (ex-args-p x)
+                      (pseudo-term-listp (ex-args->term-lst x)))))
+
+    (local (defthm lemma-2
+             (implies (and (pseudo-term-listp y) (consp y))
+                      (pseudo-termp (car y)))))
+
+    (local (defthm lemma-3
+             (implies (and (pseudo-termp z) (consp z) (not (equal (car z) 'quote)))
+                      (pseudo-term-listp (cdr z)))))
+
+    (defthm cdar-of-ex-args->term-lst-is-pseudo-term-list
+      (implies (and (ex-args-p expand-args)
+                    (consp (ex-args->term-lst expand-args))
+                    (consp (car (ex-args->term-lst expand-args)))
+                    (not (equal (caar (ex-args->term-lst expand-args)) 'quote)))
+               (pseudo-term-listp (cdar (ex-args->term-lst expand-args)))))
+
+    (local (defthm lemma-4
+             (implies (and (pseudo-term-listp y) (consp y))
+                      (pseudo-term-listp (cdr y)))))
+
+    (defthm cdr-of-ex-args->term-lst-is-pseudo-term-list
+      (implies (and (ex-args-p expand-args)
+                    (consp (ex-args->term-lst expand-args)))
+               (pseudo-term-listp (cdr (ex-args->term-lst expand-args)))))
+
+    (local (defthm lemma-5
+             (implies (and (pseudo-term-listp y) (consp y) (not (consp (car y))))
+                      (symbolp (car y)))))
+
+    (defthm symbolp-of-car-of-ex-args->term-lst
+      (implies (and (ex-args-p expand-args)
+                    (consp (ex-args->term-lst expand-args))
+                    (not (consp (car (ex-args->term-lst expand-args)))))
+               (symbolp (car (ex-args->term-lst expand-args)))))
+    )
+
+  (encapsulate ()
+    (local (in-theory (enable pseudo-lambdap)))
+
+    (defthm symbol-listp-of-formals-of-pseudo-lambdap
+      (implies (pseudo-lambdap x) (symbol-listp (cadr x))))
+
+    (defthm pseudo-termp-of-body-of-pseudo-lambdap
+      (implies (pseudo-lambdap x) (pseudo-termp (caddr x))))
+
+    (defthm consp-of-pseudo-lambdap
+      (implies (pseudo-lambdap x) (consp x)))
+
+    (defthm consp-of-cdr-of-pseudo-lambdap
+      (implies (pseudo-lambdap x) (consp (cdr x))))
+
+    (defthm consp-of-cddr-of-pseudo-lambdap
+      (implies (pseudo-lambdap x) (consp (cddr x))))
+
+    (defthm not-stringp-of-cadr-of-pseudo-lambdap
+      (implies (pseudo-lambdap x) (not (stringp (cadr x)))))
+    )
+
+  (encapsulate ()
+    (local (defthm natp-of-cdr-of-hons-get-of-ex-args->fn-lvls-of-ex-args-p
+             (implies (and (ex-args-p x) (hons-assoc-equal foo (ex-args->fn-lvls x)))
+                      (natp (cdr (hons-assoc-equal foo (ex-args->fn-lvls x)))))))
+
+    (defthm integerp-of-cdr-of-hons-get-of-ex-args->fn-lvls-of-ex-args-p
+      (implies (and (ex-args-p x) (hons-assoc-equal foo (ex-args->fn-lvls x)))
+               (integerp (cdr (hons-assoc-equal foo (ex-args->fn-lvls x)))))
+      :hints(("Goal" :use ((:instance natp-of-cdr-of-hons-get-of-ex-args->fn-lvls-of-ex-args-p (x x))))))
+
+    (defthm non-neg-of-cdr-of-hons-get-of-ex-args->fn-lvls-of-ex-args-p
+      (implies (and (ex-args-p x) (hons-assoc-equal foo (ex-args->fn-lvls x)))
+               (<= 0 (cdr (hons-assoc-equal foo (ex-args->fn-lvls x)))))
+      :hints(("Goal" :use ((:instance natp-of-cdr-of-hons-get-of-ex-args->fn-lvls-of-ex-args-p (x x)))))))
+
+  (encapsulate
+    ()
+    (set-well-founded-relation l<)
+
+    ;;
+    ;; The hypotheses each function is going to generate:
+    ;;
+    ;; If it is a non-recursive function:
+    ;;   Expanding for once should be enough.
+    ;;   Then we don't need the return types theorems.
+    ;;   Currently we are deciding that we don't need the more-returns theorems
+    ;;     for non-recursive functions.
+    ;;
+    ;; If it is a recursive function, but not declared as uninterpreted:
+    ;;   Detect it and report an error.
+    ;;
+    ;; If it is a uninterpreted function:
+    ;;   Expand it to the lowest level.
+    ;;   We need the return type theorem as auxiliary hypotheses.
+    ;;   Instantiate more returns with lambdas and the function calls.
+    ;;
+    (define expand ((expand-args ex-args-p))
+      :returns (expanded-terms pseudo-term-listp)
+      :measure (expand-measure expand-args)
+      :guard-debug t
+      :hints
+      (("Goal"
+        :use ((:instance sum-lvls-decrease-after-update
+                         (fn (car (car (ex-args->term-lst expand-args))))
+                         (fn-lvls (ex-args->fn-lvls expand-args))))))
+      :enabled t
+      (b* (;; (expand-args (mbe :logic (ex-args-fix expand-args) :exec expand-args))
+           ((unless (ex-args-p expand-args)) nil)
+           ((ex-args a) expand-args)
+           ((unless (consp a.term-lst)) nil)
+           ((cons term rest) a.term-lst)
+           ;; If first term is an atom, return the atom
+           ;; then recurse on the rest of the list
+           ((if (atom term))
+            (cons term (expand (change-ex-args expand-args :term-lst rest))))
+           ((if (and (equal (car term) 'quote)
+                     (consp (cdr term))
+                     (equal (cddr term) nil)))
+            (cons term (expand (change-ex-args expand-args :term-lst rest))))
+           ((unless (not (equal (car term) 'quote)))
+            (er hard? 'SMT-goal-generator=>expand "messed up quote: ~q0" term))
+           ;; The first term is now a function call:
+           ;; Cons the function call and function actuals out of term
+           ((cons fn-call fn-actuals) term)
+
+           ;; See if the fn-call is a lambdap:
+           (pseudo-lambda? (pseudo-lambdap fn-call))
+           ;; If it is a pseudo-lambdap
+           ((if pseudo-lambda?)
+            (b* ((lambda-formals (lambda-formals fn-call))
+                 (lambda-body (car (expand (change-ex-args expand-args :term-lst (list (lambda-body fn-call))))))
+                 (lambda-actuals (expand (change-ex-args expand-args :term-lst fn-actuals)))
+                 ((unless (equal (len lambda-formals) (len lambda-actuals)))
+                  (er hard? 'SMT-goal-generator=>expand "You called your function with the wrong number of actuals: ~q0"
+                      term)))
+              (cons `((lambda ,lambda-formals ,lambda-body) ,@lambda-actuals)
+                    (expand (change-ex-args expand-args :term-lst rest)))))
+
+           ;; If fn-call is neither a lambda expression nor a function call
+           ((unless (symbolp fn-call))
+            (er hard? 'SMT-goal-generator=>expand "Unrecognizable term: ~q0" term))
+           ;; Try finding function call from fn-lst
+           (fn (hons-get fn-call a.fn-lst))
+           ;; If fn-call doesn't exist in fn-lst, it can be a basic function,
+           ;; in that case we don't do anything with it.
+           ;; Otherwise it can be a function that's forgotten to be added to fn-lst.
+           ;; The translator will fail to translate it and report an error.
+           ((unless fn)
+            (cons (cons fn-call (expand (change-ex-args expand-args :term-lst fn-actuals)))
+                  (expand (change-ex-args expand-args :term-lst rest))))
+
+           ;; Now fn is a function in fn-lst
+           ;; If fn-call is already expanded to level 0, don't expand.
+           (lvl-item (hons-get fn-call a.fn-lvls))
+           ((unless lvl-item)
+            (er hard? 'SMT-goal-generator=>expand "Function ~q0 exists in the definition list but not in the levels list?" fn-call))
+           ((if (zp (cdr lvl-item)))
+            (cons (cons fn-call (expand (change-ex-args expand-args :term-lst fn-actuals)))
+                  (expand (change-ex-args expand-args :term-lst rest))))
+
+           ;; If fn-call is not expanded to level 0, still can expand.
+           (new-fn-lvls (update-fn-lvls fn-call a.fn-lvls))
+           ((func f) (cdr fn))
+           (formals (flatten-formals f.formals))
+           (expanded-lambda-body
+            (car (expand (change-ex-args expand-args :term-lst (list f.body) :fn-lvls new-fn-lvls))))
+           (expanded-lambda `(lambda ,formals ,expanded-lambda-body))
+           (expanded-term-list (expand (change-ex-args expand-args :term-lst fn-actuals)))
+           ((unless (equal (len formals) (len expanded-term-list)))
+            (er hard? 'SMT-goal-generator=>expand "You called your function with the wrong number of actuals: ~q0"
+                term))
+           )
+        (cons `(,expanded-lambda ,@expanded-term-list)
+              (expand (change-ex-args expand-args :term-lst rest))))
+      )
+    )
+
+  (defthm pseudo-termp-of-car-of-expand
+    (implies (ex-args-p expand-args)
+             (pseudo-termp (car (expand expand-args)))))
+
+  (define initialize-fn-lvls ((fn-lst func-alistp))
+    :returns (fn-lvls sym-nat-alistp)
+    :enabled t
+    (b* (((unless (func-alistp fn-lst)) nil)
+         ((unless (consp fn-lst)) nil)
+         ((cons first rest) fn-lst)
+         ((func f) (cdr first)))
+      (cons (cons f.name f.expansion-depth) (initialize-fn-lvls rest))))
+
+  ;; Generate auxiliary hypotheses from the user given hypotheses
+  (define generate-hyp-hint-lst ((hyp-lst hint-pair-listp) (fn-lst func-alistp) (fn-lvls sym-nat-alistp))
     :returns (hyp-hint-lst hint-pair-listp)
-    :ignore-ok t
-    :irrelevant-formals-ok t
+    (b* (((if (endp hyp-lst)) nil)
+         ((cons (hint-pair hyp) rest) hyp-lst)
+         (G-prim (car (expand (make-ex-args :term-lst (list hyp.thm)
+                                            :fn-lst fn-lst
+                                            :fn-lvls fn-lvls)))))
+      (cons (make-hint-pair :thm G-prim
+                            :hints hyp.hints)
+            (generate-hyp-hint-lst rest fn-lst fn-lvls))))
 
-    nil
-    )
+  ;; (define generate-fn-hint-pair ((hypo hint-pair-p)
+  ;;                                (fn-name symbolp) (returns symbol-listp) (formals symbol-listp)
+  ;;                                (actuals pseudo-term-listp))
+  ;;   :returns (fn-hint-pair hint-pair-p)
+  ;;   (b* (((hint-pair p) hypo)
+  ;;        (free-vars (all-vars p.thm))
+  ;;        ;; If the returns theorems contain free variables,
+  ;;        ;; report an error.
+  ;;        ((unless (subsetp free-vars (append returns formals)))
+  ;;         (er hard? 'SMT-goal-generator=>generate-fn-hint-pair "Function returns theorem contain free variables: ~q0. The formals are: ~q1 and the returns are: ~q2." p.thm formals returns)))
+  ;;     `((lambda ,formals ((lambda ,returns ,p.thm) (,fn-name ,@formals))) ,@actuals)))
 
-  (define SMT-goal-generator (cl hints)
-    :guard (and (smtlink-hint-p hints)
-                (pseudo-term-listp cl))
+  ;; (define generate-fn-returns-hint ((returns decl-listp) (fn-name symbolp)
+  ;;                                   (formals decl-listp) (actuals pseudo-term-listp)
+  ;;                                   (fn-hint-acc hint-pair-listp))
+  ;;   :returns (fn-hint-lst hint-pair-listp :hyp :guard)
+  ;;   :ignore-ok t
+  ;;   nil)
+
+  ;; (define generate-fn-more-returns-hint ((more-returns hint-pair-listp) (fn-name symbolp)
+  ;;                                        (formals decl-listp) (actuals pseudo-term-listp)
+  ;;                                        (fn-hint-acc hint-pair-listp))
+  ;;   :returns (fn-hint-lst hint-pair-listp :hyp :guard)
+  ;;   :ignore-ok t
+  ;;   nil)
+
+  ;; (define generate-fn-hint ((fn func-p) (fn-actuals pseudo-term-listp)
+  ;;                           (fn-hint-acc hint-pair-listp))
+  ;;   :returns (fn-hint-lst hint-pair-listp :hyp :guard)
+  ;;   (b* (((func f) fn)
+  ;;        ((unless f.uninterpreted)
+  ;;         (er hard? 'SMT-goal-generator=>generate-fn-hint "Function call ~q0 still exists in term but it's not declared as an uninterpreted function." f.name))
+  ;;        (new-fn-hint-acc
+  ;;         (generate-fn-returns-hint f.returns f.name f.formals fn-actuals fn-hint-acc)))
+  ;;     (generate-fn-more-returns-hint f.more-returns f.name f.formals fn-actuals new-fn-hint-acc)))
+
+
+  ;; ;; function hypotheses generation arguments
+  ;; (defprod fhg-args
+  ;;   ((term-lst pseudo-term-listp :default nil)
+  ;;    (fn-lst func-alistp :default nil)
+  ;;    (fn-hint-acc hint-pair-listp :default nil)))
+
+  ;; ;; Generate auxiliary hypotheses from function expansion
+  ;; (define generate-fn-hint-lst ((args fhg-args-p))
+  ;;   :returns (fn-hint-lst hint-pair-listp)
+  ;;   (b* (;; If guard is violated, return nil
+  ;;        ((unless (fhg-args-p args)) nil)
+  ;;        ;; Bind the fields out of the defprod type
+  ;;        ((fhg-args a) args)
+  ;;        ;; If a.term-lst is nil,
+  ;;        ;; return the function hint accumulator a.fn-hint-acc
+  ;;        ((unless (consp a.term-lst)) a.fn-hint-acc)
+  ;;        ;; If not,
+  ;;        ;; cons the first element out of a.term-lst
+  ;;        ((cons first rest) a.term-lst)
+
+  ;;        ;; If first is symbolp, don't need to generate any hypo
+  ;;        ((if (symbolp first))
+  ;;         (generate-fn-hint-lst (change-fhg-args :term-lst rest)))
+  ;;        ;; Else it must be a consp, if it is a quoted thingy
+  ;;        ;; The quoted thingy (cadr term) can be a non-pseudo-termp.
+  ;;        ((if (and (equal (car term) 'quote)
+  ;;                  (consp (cdr term))
+  ;;                  (equal (cddr term) nil)))
+  ;;         (generate-fn-hint-lst (change-fhg-args :term-lst rest)))
+
+  ;;        ;; Now first must be a true-listp
+  ;;        ((cons fn-call fn-actuals) first)
+
+  ;;        ;; If term is an atom, return fn-hint-acc
+  ;;        ((if (atom G-prim)) fn-hint-acc)
+  ;;        ;; If term is nil, return fn-hint-acc
+  ;;        ((if (endp G-prim)) fn-hint-acc)
+  ;;        ;; Cons the function call and function actuals out of term
+  ;;        ((cons fn-call fn-actuals) term)
+  ;;        ;; See if fn-call is a lambda expression
+  ;;        (pseudo-lambda? (pseudo-lambdap fn-call))
+  ;;        ;; Try finding function call from fn-lst
+  ;;        (fn (hons-get fn-call fn-lst))
+  ;;        ;; If fn-call does not belong to fn-lst and it is not a lambda,
+  ;;        ;; then no need to add any hypotheses.
+  ;;        ((unless (or fn pseudo-lambda?))
+  ;;         (generate-fn-hint-lst-on-lst fn-actuals fn-lst fn-hint-acc))
+  ;;        ;; If fn-call belongs to fn-lst
+  ;;        ((if fn)
+  ;;         (generate-fn-hint-lst-on-lst fn-actuals fn-lst
+  ;;                                      (generate-fn-hint (cdr fn) fn-actuals fn-hint-acc)))
+  ;;        ;; Else fn-call is a lambda expression
+  ;;        (body-fn-hint-lst (generate-fn-hint-lst (lambda-body fn-call) fn-lst fn-hint-acc))
+  ;;        )
+  ;;     (generate-fn-hint-lst-on-lst fn-actuals fn-lst body-fn-hint-lst)))
+
+  ;; Make fn-lst a fast alist
+  (define make-alist-fn-lst ((fn-lst func-listp))
+    :returns (fast-fn-lst func-alistp)
+    :measure (len fn-lst)
+    :enabled t
+    (b* ((fn-lst (mbe :logic (func-list-fix fn-lst) :exec fn-lst))
+         ((unless (consp fn-lst)) nil)
+         ((cons first rest) fn-lst)
+         ((func f) first))
+      (cons (cons f.name f) (make-alist-fn-lst rest))))
+
+  ;; The top level function for generating SMT goals: G-prim and A's
+  (define SMT-goal-generator ((cl pseudo-term-listp) (hints smtlink-hint-p))
     :returns (new-hints smtlink-hint-p)
+    :short "@(call SMT-goal-generator) is the top level function for generating SMT goals: G-prim and A's"
 
-    (b* ((fn-lst (smtlink-hint->functions hints))
-         (fn-hint-lst (generate-fn-hint-lst fn-lst))
+    (b* ((cl (mbe :logic (pseudo-term-list-fix cl) :exec cl))
+         (hints (mbe :logic (smtlink-hint-fix hints) :exec hints))
+         ((smtlink-hint h) hints)
+         ;; Make a fast alist version of fn-lst
+         (fn-lst (make-alist-fn-lst h.functions))
+         (fn-lvls (initialize-fn-lvls fn-lst))
 
-         (hyp-lst (smtlink-hint->hypotheses hints))
-         (hyp-hint-lst (generate-hyp-hint-lst hyp-lst))
+         ;; Generate user given hypotheses and their hints from hyp-lst
+         (hyp-hint-lst (with-fast-alist fn-lst (generate-hyp-hint-lst h.hypotheses fn-lst fn-lvls)))
 
-         (total-aux-hint-lst `(,@(fn-hint-lst hyp-hint-lst)))
+         ;; Expand main clause using fn-lst
+         ;; Generate function hypotheses and their hints from fn-lst
+         (G-prim
+          (with-fast-alist fn-lst (car (expand (make-ex-args
+                                                :term-lst (list (disjoin cl))
+                                                :fn-lst fn-lst
+                                                :fn-lvls fn-lvls)))))
 
-         (G-prim (expand (disjoin cl) fn-lst))
-         (main-hint (smtlink-hint->main-hint hints))
-         (expanded-clause-w/-hint `(G-prim . main-hint))
+         ;; Generate auxiliary hypotheses from function expansion
+         (fn-hint-lst ;; (generate-fn-hint-lst G-prim fn-lst nil)
+          nil)
+
+         ;; Combine all auxiliary hypotheses
+         (total-aux-hint-lst `(,@fn-hint-lst ,@hyp-hint-lst))
+
+         ;; Combine expanded main clause and its hint
+         (expanded-clause-w/-hint (make-hint-pair :thm G-prim :hints h.main-hint))
+
+         ;; Update smtlink-hint
          (new-hints
           (change-smtlink-hint hints
+                               :fast-functions fn-lst
                                :aux-hint-list total-aux-hint-lst
                                :expanded-clause-w/-hint expanded-clause-w/-hint
                                )))
