trusted/SMT-prove.lisp
@@ -9,38 +9,41 @@
 (include-book "../verified/SMT-hint-interface")
 (include-book "../verified/SMT-config")
 
-(defun mk-fname (directory fname-LISP suffix)
-  (let ((dir (if (equal directory "") "/tmp/py_file" directory)))
-    (cond ((equal fname-LISP "")
-           (let ((cmd (concatenate 'string "mkdir -p " dir " && "
-                                   "mktemp " dir "/smtlink" suffix ".XXXXX")))
-             (mv-let (exit-status lines)
-               (time$ (tshell-call cmd
-                                   :print t
-                                   :save t)
-                      :msg "; mktemp: `~s0`: ~st sec, ~sa bytes~%"
-                      :args (list cmd))
-               (if (equal exit-status 0)
-                   (car lines)
-                 (er hard? 'top-level "Error: Generate file error.")))))
-          ((stringp fname-LISP)
-           (concatenate 'string dir "/" (string (lisp-to-python-names fname-LISP)) suffix))
-          (t (er hard? 'top-level "Error: fname should either be a string or \"\"")))))
+;; (defun mk-fname (directory fname-LISP suffix)
+;;   (let ((dir (if (equal directory "") "/tmp/py_file" directory)))
+;;     (cond ((equal fname-LISP "")
+;;            (let ((cmd (concatenate 'string "mkdir -p " dir " && "
+;;                                    "mktemp " dir "/smtlink" suffix ".XXXXX")))
+;;              (mv-let (exit-status lines)
+;;                (time$ (tshell-call cmd
+;;                                    :print t
+;;                                    :save t)
+;;                       :msg "; mktemp: `~s0`: ~st sec, ~sa bytes~%"
+;;                       :args (list cmd))
+;;                (if (equal exit-status 0)
+;;                    (car lines)
+;;                  (er hard? 'top-level "Error: Generate file error.")))))
+;;           ((stringp fname-LISP)
+;;            (concatenate 'string dir "/" (string (lisp-to-python-names fname-LISP)) suffix))
+;;           (t (er hard? 'top-level "Error: fname should either be a string or \"\"")))))
 
-(defun write-SMT-file (py-term smt-file)
-  (declare (ignore py-term smt-file))
-  )
+;; (defun write-SMT-file (py-term smt-file)
+;;   (declare (ignore py-term smt-file))
+;;   )
 
-(defun SMT-prove (term)
-  (b* ((fname (smtlink-hint->python-file (smt-hint)))
-       (uninterpreted (smtlink-hint->uninterpreted (smt-hint)))
-       (directory (smtlink-config->SMT-files-dir (smt-cnf)))
-       (file-format (smtlink-config->file-format (smt-cnf)))
-       (smt-file (mk-fname directory fname file-format))
+;; (defun SMT-prove (term)
+;;   (b* ((fname (smtlink-hint->python-file (smt-hint)))
+;;        (uninterpreted (smtlink-hint->uninterpreted (smt-hint)))
+;;        (directory (smtlink-config->SMT-files-dir (smt-cnf)))
+;;        (file-format (smtlink-config->file-format (smt-cnf)))
+;;        (smt-file (mk-fname directory fname file-format))
 
-       (translated-py-term (SMT-transliteration term))
+;;        (translated-py-term (SMT-transliteration term))
 
-       (state (write-SMT-file translated-py-term smt-file))
+;;        (state (write-SMT-file translated-py-term smt-file))
 
-       (result (run-SMT-solver smt-file))))
-  result)
+;;        (result (run-SMT-solver smt-file))))
+;;   result)
+
+(define SMT-prove (term)
+  (or term t))
